Surface/Examples/Boolean.lean
@@ -13,8 +13,8 @@ def benv : GlobalEnv := [
 
   -- .instDecl "EqBoolI" ⟨1, #(`★), 0, #(), 1, #(gt`#"Bool"), gt`#"Eq" `• t`#0⟩ #(("eq", λˢ[gt`#"Bool"] λˢ[gt`#"Bool"] `#0)),
   -- .classDecl "Eq" #(`★) #() #() #(("eq",  ⟨0, #(), 0, #(), 0, #(), t`#0 `-:> (t`#0 `-:> gt`#"Bool")⟩)),
-  .data (n := 2) "Bool" `★ #(("True", ⟨0, #(), 0, #(), 0,  #(), gt`#"Bool"⟩),
-                             ("False", ⟨0, #(), 0, #(), 0, #(), gt`#"Bool"⟩))
+  .data (n := 2) "Bool" ★ #(("True", ⟨0, #(), 0, #(), 0,  #(), gt#"Bool"⟩),
+                            ("False", ⟨0, #(), 0, #(), 0, #(), gt#"Bool"⟩))
   ]
 
 #eval benv
