Surface/Global.lean
@@ -1,7 +1,7 @@
 import LeanSubst
 import Core.Vec
 import Lilac
-import Surface.Ty
+-- import Surface.Ty
 import Surface.Term
 
 open LeanSubst
@@ -10,20 +10,20 @@ open Lilac
 namespace Surface
 
 inductive Global where
-| data : {n : Nat} -> String -> Kind -> Vec (String × SpineTy) n -> Global
-| defn : String -> Ty -> Term -> Global
+| data : {n : Nat} -> String -> Core.Kind -> Vec (String × Core.SpineTy) n -> Global
+| defn : String -> Core.Ty -> Term -> Global
 | classDecl : {kc : Nat} ->
-  String -> Vec Kind kc -> -- TODO Change Vec to List for SC and determiners of FDs and methods
+  String -> Vec Core.Kind kc -> -- TODO Change Vec to List for SC and determiners of FDs and methods
   List (String × String × List (Fin kc)) ->
   List (String × (n : Nat) × Vec (Fin kc) (n + 1) × Fin kc) ->
-  List (String × SpineTy) -> Global
-| instDecl : String -> SpineTy -> List (String × Term) -> Global  -- what to do with instance constraints and ty params?
+  List (String × Core.SpineTy) -> Global
+| instDecl : String -> Core.SpineTy -> List (String × Term) -> Global  -- what to do with instance constraints and ty params?
 
 
 def Global.repr (_ : Nat) : (a : Global) -> Std.Format
 | .data s K ctors =>
   (Std.Format.text ".data ") ++ (Std.Format.text s) ++ " : "
-    ++ (Kind.repr max_prec K) ++ (Std.Format.text " where ") ++
+    ++ (K.repr max_prec) ++ (Std.Format.text " where ") ++
     Std.Format.line ++ Std.Format.nest 4 (ctors.reprPrec 0)
 | .defn n T t => ".defn " ++ n ++ " " ++ (T.repr max_prec) ++ t.repr max_prec
 | classDecl s Ks scs fds methods =>
@@ -31,7 +31,7 @@ def Global.repr (_ : Nat) : (a : Global) -> Std.Format
     ++ "|" ++ fds.repr max_prec ++ (Std.Format.text " where ")
     ++ Std.Format.line ++ (methods.repr max_prec)
 | instDecl i_name spTy methods =>
-  (Std.Format.text ".inst ") ++ i_name ++ " : " ++ "⟨" ++ spTy.repr max_prec ++ "⟩"
+  (Std.Format.text ".inst ") ++ i_name ++ " : " ++ "⟨" ++ spTy.repr ++ "⟩"
     ++ Std.Format.line ++ Std.Format.nest 4 (methods.repr max_prec)
 
 @[simp]
@@ -42,12 +42,12 @@ instance instRepr_Global : Repr (Global) where
 abbrev GlobalEnv := List (Global)
 
 inductive Entry : Type where
-| data : {n : Nat} -> String -> Kind -> Vec (String × SpineTy) n -> Entry
-| ctor : String -> Nat -> SpineTy -> Entry
-| defn : String -> Ty -> Term -> Entry
-| odata : {n : Nat} -> String -> Vec Kind n -> Entry
-| octor : String -> SpineTy -> Entry
-| openm : String -> SpineTy -> Entry
+| data : {n : Nat} -> String -> Core.Kind -> Vec (String × Core.SpineTy) n -> Entry
+| ctor : String -> Nat -> Core.SpineTy -> Entry
+| defn : String -> Core.Ty -> Term -> Entry
+| odata : {n : Nat} -> String -> Vec Core.Kind n -> Entry
+| octor : String -> Core.SpineTy -> Entry
+| openm : String -> Core.SpineTy -> Entry
 
 def Entry.is_data : Entry -> Bool
 | data _ _ _ => true
@@ -69,9 +69,9 @@ def Entry.is_defn : Entry -> Bool
 | defn _ _ _ => true
 | _ => false
 
-def Entry.kind : Entry -> Option Kind
+def Entry.kind : Entry -> Option Core.Kind
 | data _ K _ => K
-| odata _ Ks => Kind.mk_kind Ks
+| odata _ Ks => Core.Kind.mk_kind Ks
 | _ => none
 
 
@@ -86,10 +86,10 @@ def lookup (x : String) : GlobalEnv -> Option (Entry)
 | .cons (.defn y a b) tl =>
   if x == y then return .defn y a b else lookup x tl
 | .cons (.classDecl (kc := kc) y Ks scs fds ms) tl =>
-  let ms_mb : Option (String × SpineTy) := ms.find? (λ (mn, _) => x == mn)
+  let ms_mb : Option (String × Core.SpineTy) := ms.find? (λ (mn, _) => x == mn)
   let ms := ms_mb.map (λ (x, mn) => .openm x mn)
   let scs_mb : Option (String × String × List (Fin kc)) := scs.find? (λ (sc, _, _) => x == sc)
-  let scs := scs_mb.map (λ (scn, cls, tys) => .openm scn ⟨kc, Ks, 0, #(), 1, #((gt`#y).mkApps_nats (List.range kc)), (gt`#cls).mkApps_nats tys⟩ )
+  let scs := scs_mb.map (λ (scn, cls, tys) => .openm scn ⟨kc, Ks, 0, #(), 1, #((gt#y).mkApps_nats (List.range kc)), (gt#cls).mkApps_nats tys⟩ )
   -- let fds_mb : Option (String × (n : Nat) × Vec (Fin kc) (n + 1) × Fin kc) := fds.find? (λ ⟨fdn, _, _, _⟩ => x == fdn)
   -- let fds := fds_mb.map (λ ⟨fdn, n, dns, dt⟩ => Entry.openm fdn ⟨kc, Ks, 0, #(), 2, #(sorry, sorry), t`#0 ⟩)
   if x == y then return .odata y Ks
@@ -101,7 +101,7 @@ def lookup (x : String) : GlobalEnv -> Option (Entry)
   if x == s then return .octor s spTy
   else lookup x tl
 
-def lookup_kind (G : GlobalEnv) (x : String) : Option Kind := lookup x G |> Option.map Entry.kind |> Option.get!
+def lookup_kind (G : GlobalEnv) (x : String) : Option Core.Kind := lookup x G |> Option.map Entry.kind |> Option.get!
 
 
 -- def is_ctor (G : GlobalEnv) x := lookup x G |> Option.map Entry.is_ctor |> Option.get!
