Surface/Ty.lean
@@ -1,4 +1,4 @@
-import Surface.Ty.Definition
-import Surface.Ty.BEq
-import Surface.Ty.Substitution
-import Surface.Ty.Structure
+-- import Surface.Ty.Definition
+-- import Surface.Ty.BEq
+-- import Surface.Ty.Substitution
+-- import Surface.Ty.Structure
