Surface/Typing.lean
@@ -1,7 +1,7 @@
 import LeanSubst
 import Core.Vec
 
-import Surface.Ty
+-- import Surface.Ty
 import Surface.Term
 import Surface.Global
 
@@ -9,68 +9,68 @@ import Surface.Global
 namespace Surface
 
 @[simp]
-abbrev KindEnv := List Kind
+abbrev KindEnv := List Core.Kind
 
 @[simp]
-abbrev TyEnv := List Ty
+abbrev TyEnv := List Core.Ty
 
 
-inductive Kinding (G : GlobalEnv) : KindEnv -> Ty -> Kind -> Prop
+inductive Kinding (G : GlobalEnv) : KindEnv -> Core.Ty -> Core.Kind -> Prop
 | var :
   Δ[x]? = some K ->
-  Kinding G Δ t`#x K
+  Kinding G Δ t#x K
 | global :
   lookup_kind G x = some K ->
-  Kinding G Δ gt`#x K
+  Kinding G Δ gt#x K
 | arrow :
-  Kinding G Δ A `★ ->
-  Kinding G Δ B (.base b2) ->
-  Kinding G Δ (A `-:> B) `★
-| «then» :
-  Kinding G Δ A `◯ ->
-  Kinding G Δ B (.base b2) ->
-  Kinding G Δ (A `=:> B) `★
+  Kinding G Δ A ★ ->
+  Kinding G Δ B ★ ->
+  Kinding G Δ (A -:> B) ★
+-- | «then» :
+--   Kinding G Δ A ★ ->
+--   Kinding G Δ B (.base b2) ->
+--   Kinding G Δ (A `=:> B) `★
 | all :
-  Kinding G (K::Δ) P `★ ->
-  Kinding G Δ (`∀[K] P) `★
+  Kinding G (K::Δ) P ★ ->
+  Kinding G Δ (∀[K] P) ★
 | app :
-  Kinding G Δ f (A `-:> B) ->
+  Kinding G Δ f (A -:> B) ->
   Kinding G Δ a A ->
-  Kinding G Δ (f `• a) B
+  Kinding G Δ (f • a) B
 
 
 notation:170 G:170 "&" Δ:170 " ⊢s " A:170 " : " K:170 => Kinding G Δ A K
 
-inductive ValidCtor (x : String) : Ty -> Prop where
+inductive ValidCtor (x : String) : Core.Ty -> Prop where
 | base :
   T.spine = some (x, sp) ->
   ValidCtor x T
 | all :
   ValidCtor x P ->
-  ValidCtor x (`∀[K] P)
+  ValidCtor x (∀[K] P)
 | arrow :
   ValidCtor x B ->
-  ValidCtor x (A `-:> B)
+  ValidCtor x (A -:> B)
 
 -- Valid Class Methods are of the form
 -- ∀αs (x βs) => B
-inductive ValidClassMethodTy (x : String) : Ty -> Prop where
-| base :
-  T.spine = some (x, sp) ->
-  ValidClassMethodTy x T
-| all :
-  ValidClassMethodTy x P ->
-  ValidClassMethodTy x (`∀[K] P)
-| arrow :
-  A.spine = some (x, sp) ->
-  ValidClassMethodTy x (A `=:> B)
+-- inductive ValidClassMethodTy (x : String) : Core.Ty -> Prop where
+-- | base :
+--   T.spine = some (x, sp) ->
+--   ValidClassMethodTy x T
+-- | all :
+--   ValidClassMethodTy x P ->
+--   ValidClassMethodTy x (∀[K] P)
+-- | arrow :
+--   A.spine = some (x, sp) ->
+--   ValidClassMethodTy x (A `=:> B)
 
-inductive ValidOpenKind : Kind -> Prop where
-| base : ValidOpenKind `◯
-| arrow : ValidOpenKind B -> ValidOpenKind (A `-:> B)
+-- inductive ValidOpenKind : Kind -> Prop where
+-- | base : ValidOpenKind `◯
+-- | arrow : ValidOpenKind B -> ValidOpenKind (A `-:> B)
 
 
-inductive ValidClassInstTy (x : String) : Ty -> Prop where
+inductive ValidClassInstTy (x : String) : Core.Ty -> Prop where
 | base :
   T.spine = some (x, sp) ->
   ValidClassInstTy x T
