Translation.lean
@@ -1,7 +1,7 @@
 import Core.Ty
-import Surface.Ty
+-- import Surface.Ty
 
-import Translation.Ty
+-- import Translation.Ty
 import Translation.Term
 import Translation.Global
 
